theories/IndTypes/Syntax.v
@@ -74,235 +74,226 @@ Inductive gType  : Set :=
   | GBranch : action -> seq gType -> gType  
  with value  : Set  :=
   | VSeqSort : seq mysort -> value  
-  | VLT : endpoint -> ptcp  -> value  
+  | VLT : lType -> ptcp  -> value  
  with mysort  : Set :=
   | SBool : mysort
   | SNat : mysort  
   | SGType : gType -> mysort (*maybe more sorts?*)
- with endpoint  : Set :=
-  | EVar : nat -> endpoint  
-  | EEnd : endpoint  
-  | EMsg : dir -> ch -> value -> endpoint -> endpoint  
-  | EBranch  : dir -> ch  -> seq endpoint -> endpoint  
-  | ERec : endpoint -> endpoint . 
+ with lType  : Set :=
+  | EVar : nat -> lType  
+  | EEnd : lType  
+  | EMsg : dir -> ch -> value -> lType -> lType  
+  | EBranch  : dir -> ch  -> seq lType -> lType  
+  | ERec : lType -> lType . 
 Set Elimination Schemes.
 
-Section endpoint.
+Section lType.
 
 
 Lemma congr_EEnd  : EEnd  = EEnd  .
 Proof. congruence. Qed.
 
-Lemma congr_ERec  { s0 : endpoint   } { t0 : endpoint   } (H1 : s0 = t0) : ERec  s0 = ERec  t0 .
+Lemma congr_ERec  { s0 : lType   } { t0 : lType   } (H1 : s0 = t0) : ERec  s0 = ERec  t0 .
 Proof. congruence. Qed.
 
-Lemma congr_EMsg  { s0 : dir   } { s1 : ch   } { s2 : value   } { s3 : endpoint   } { t0 : dir   } { t1 : ch   } { t2 : value   } { t3 : endpoint   } (H1 : s0 = t0) (H2 : s1 = t1) (H3 : s2 = t2) (H4 : s3 = t3) : EMsg  s0 s1 s2 s3 = EMsg  t0 t1 t2 t3 .
+Lemma congr_EMsg  { s0 : dir   } { s1 : ch   } { s2 : value   } { s3 : lType   } { t0 : dir   } { t1 : ch   } { t2 : value   } { t3 : lType   } (H1 : s0 = t0) (H2 : s1 = t1) (H3 : s2 = t2) (H4 : s3 = t3) : EMsg  s0 s1 s2 s3 = EMsg  t0 t1 t2 t3 .
 Proof. congruence. Qed.
 
-Lemma congr_EBranch  { s0 : dir   } { s1 : ch   } { s2 : list (endpoint  ) } { t0 : dir   } { t1 : ch   } { t2 : list (endpoint  ) } (H1 : s0 = t0) (H2 : s1 = t1) (H3 : s2 = t2) : EBranch  s0 s1 s2 = EBranch  t0 t1 t2 .
+Lemma congr_EBranch  { s0 : dir   } { s1 : ch   } { s2 : list (lType  ) } { t0 : dir   } { t1 : ch   } { t2 : list (lType  ) } (H1 : s0 = t0) (H2 : s1 = t1) (H3 : s2 = t2) : EBranch  s0 s1 s2 = EBranch  t0 t1 t2 .
 Proof. congruence. Qed.
 
-Definition upRen_endpoint_endpoint   (xi : ( fin ) -> fin) : ( fin ) -> fin :=
+Definition upRen_lType_lType   (xi : ( fin ) -> fin) : ( fin ) -> fin :=
   (up_ren) xi.
 
-Fixpoint ren_endpoint   (xiendpoint : ( fin ) -> fin) (s : endpoint ) : endpoint  :=
-    match s return endpoint  with
-    | EVar  s => (EVar ) (xiendpoint s)
+Fixpoint ren_lType   (xilType : ( fin ) -> fin) (s : lType ) : lType  :=
+    match s return lType  with
+    | EVar  s => (EVar ) (xilType s)
     | EEnd   => EEnd 
-    | ERec  s0 => ERec  ((ren_endpoint (upRen_endpoint_endpoint xiendpoint)) s0)
-    | EMsg  s0 s1 s2 s3 => EMsg  ((fun x => x) s0) ((fun x => x) s1) ((fun x => x) s2) ((ren_endpoint xiendpoint) s3)
-    | EBranch  s0 s1 s2 => EBranch  ((fun x => x) s0) ((fun x => x) s1) ((map (ren_endpoint xiendpoint)) s2)
+    | ERec  s0 => ERec  ((ren_lType (upRen_lType_lType xilType)) s0)
+    | EMsg  s0 s1 s2 s3 => EMsg  ((fun x => x) s0) ((fun x => x) s1) ((fun x => x) s2) ((ren_lType xilType) s3)
+    | EBranch  s0 s1 s2 => EBranch  ((fun x => x) s0) ((fun x => x) s1) ((map (ren_lType xilType)) s2)
     end.
 
-Definition up_endpoint_endpoint   (sigma : ( fin ) -> endpoint ) : ( fin ) -> endpoint  :=
-  (scons) ((EVar ) (var_zero)) ((funcomp) (ren_endpoint (shift)) sigma).
+Definition up_lType_lType   (sigma : ( fin ) -> lType ) : ( fin ) -> lType  :=
+  (scons) ((EVar ) (var_zero)) ((funcomp) (ren_lType (shift)) sigma).
 
-Fixpoint subst_endpoint   (sigmaendpoint : ( fin ) -> endpoint ) (s : endpoint ) : endpoint  :=
-    match s return endpoint  with
-    | EVar  s => sigmaendpoint s
+Fixpoint subst_lType   (sigmalType : ( fin ) -> lType ) (s : lType ) : lType  :=
+    match s return lType  with
+    | EVar  s => sigmalType s
     | EEnd   => EEnd 
-    | ERec  s0 => ERec  ((subst_endpoint (up_endpoint_endpoint sigmaendpoint)) s0)
-    | EMsg  s0 s1 s2 s3 => EMsg  ((fun x => x) s0) ((fun x => x) s1) ((fun x => x) s2) ((subst_endpoint sigmaendpoint) s3)
-    | EBranch  s0 s1 s2 => EBranch  ((fun x => x) s0) ((fun x => x) s1) ((map (subst_endpoint sigmaendpoint)) s2)
+    | ERec  s0 => ERec  ((subst_lType (up_lType_lType sigmalType)) s0)
+    | EMsg  s0 s1 s2 s3 => EMsg  ((fun x => x) s0) ((fun x => x) s1) ((fun x => x) s2) ((subst_lType sigmalType) s3)
+    | EBranch  s0 s1 s2 => EBranch  ((fun x => x) s0) ((fun x => x) s1) ((map (subst_lType sigmalType)) s2)
     end.
 
 
 
 
-Definition upId_endpoint_endpoint  (sigma : ( fin ) -> endpoint ) (Eq : forall x, sigma x = (EVar ) x) : forall x, (up_endpoint_endpoint sigma) x = (EVar ) x :=
+Definition upId_lType_lType  (sigma : ( fin ) -> lType ) (Eq : forall x, sigma x = (EVar ) x) : forall x, (up_lType_lType sigma) x = (EVar ) x :=
   fun n => match n with
-  | S fin_n => (ap) (ren_endpoint (shift)) (Eq fin_n)
+  | S fin_n => (ap) (ren_lType (shift)) (Eq fin_n)
   | 0  => Logic.eq_refl
   end.
 
 
-Fixpoint idSubst_endpoint  (sigmaendpoint : ( fin ) -> endpoint ) (Eqendpoint : forall x, sigmaendpoint x = (EVar ) x) (s : endpoint ) : subst_endpoint sigmaendpoint s = s :=
-    match s return subst_endpoint sigmaendpoint s = s with
-    | EVar  s => Eqendpoint s
+Fixpoint idSubst_lType  (sigmalType : ( fin ) -> lType ) (EqlType : forall x, sigmalType x = (EVar ) x) (s : lType ) : subst_lType sigmalType s = s :=
+    match s return subst_lType sigmalType s = s with
+    | EVar  s => EqlType s
     | EEnd   => congr_EEnd 
-    | ERec  s0 => congr_ERec ((@idSubst_endpoint (up_endpoint_endpoint sigmaendpoint) (@upId_endpoint_endpoint (_) Eqendpoint)) s0)
-    | EMsg  s0 s1 s2 s3 => congr_EMsg ((fun x => (Logic.eq_refl) x) s0) ((fun x => (Logic.eq_refl) x) s1) ((fun x => (Logic.eq_refl) x) s2) ((@idSubst_endpoint sigmaendpoint  Eqendpoint) s3)
-    | EBranch  s0 s1 s2 => congr_EBranch ((fun x => (Logic.eq_refl) x) s0) ((fun x => (Logic.eq_refl) x) s1) ((list_id (@idSubst_endpoint sigmaendpoint Eqendpoint)) s2)
+    | ERec  s0 => congr_ERec ((@idSubst_lType (up_lType_lType sigmalType) (@upId_lType_lType (_) EqlType)) s0)
+    | EMsg  s0 s1 s2 s3 => congr_EMsg ((fun x => (Logic.eq_refl) x) s0) ((fun x => (Logic.eq_refl) x) s1) ((fun x => (Logic.eq_refl) x) s2) ((@idSubst_lType sigmalType  EqlType) s3)
+    | EBranch  s0 s1 s2 => congr_EBranch ((fun x => (Logic.eq_refl) x) s0) ((fun x => (Logic.eq_refl) x) s1) ((list_id (@idSubst_lType sigmalType EqlType)) s2)
     end.
 
 
 
-Definition upExtRen_endpoint_endpoint   (xi : ( fin ) -> fin) (zeta : ( fin ) -> fin) (Eq : forall x, xi x = zeta x) : forall x, (upRen_endpoint_endpoint xi) x = (upRen_endpoint_endpoint zeta) x :=
+Definition upExtRen_lType_lType   (xi : ( fin ) -> fin) (zeta : ( fin ) -> fin) (Eq : forall x, xi x = zeta x) : forall x, (upRen_lType_lType xi) x = (upRen_lType_lType zeta) x :=
   fun n => match n with
   | S fin_n => (ap) (shift) (Eq fin_n)
   | 0  => Logic.eq_refl
   end.
 
 
-Fixpoint extRen_endpoint   (xiendpoint : ( fin ) -> fin) (zetaendpoint : ( fin ) -> fin) (Eqendpoint : forall x, xiendpoint x = zetaendpoint x) (s : endpoint ) : ren_endpoint xiendpoint s = ren_endpoint zetaendpoint s :=
-    match s return ren_endpoint xiendpoint s = ren_endpoint zetaendpoint s with
-    | EVar  s => (ap) (EVar ) (Eqendpoint s)
+Fixpoint extRen_lType   (xilType : ( fin ) -> fin) (zetalType : ( fin ) -> fin) (EqlType : forall x, xilType x = zetalType x) (s : lType ) : ren_lType xilType s = ren_lType zetalType s :=
+    match s return ren_lType xilType s = ren_lType zetalType s with
+    | EVar  s => (ap) (EVar ) (EqlType s)
     | EEnd   => congr_EEnd 
-    | ERec  s0 => congr_ERec ((@extRen_endpoint (upRen_endpoint_endpoint xiendpoint) (upRen_endpoint_endpoint zetaendpoint) (@upExtRen_endpoint_endpoint (_) (_) Eqendpoint)) s0)
-    | EMsg  s0 s1 s2 s3 => congr_EMsg ((fun x => (Logic.eq_refl) x) s0) ((fun x => (Logic.eq_refl) x) s1) ((fun x => (Logic.eq_refl) x) s2) ((@extRen_endpoint xiendpoint zetaendpoint Eqendpoint) s3)
-    | EBranch  s0 s1 s2 => congr_EBranch ((fun x => (Logic.eq_refl) x) s0) ((fun x => (Logic.eq_refl) x) s1) ((list_ext (@extRen_endpoint xiendpoint zetaendpoint Eqendpoint)) s2)
+    | ERec  s0 => congr_ERec ((@extRen_lType (upRen_lType_lType xilType) (upRen_lType_lType zetalType) (@upExtRen_lType_lType (_) (_) EqlType)) s0)
+    | EMsg  s0 s1 s2 s3 => congr_EMsg ((fun x => (Logic.eq_refl) x) s0) ((fun x => (Logic.eq_refl) x) s1) ((fun x => (Logic.eq_refl) x) s2) ((@extRen_lType xilType zetalType EqlType) s3)
+    | EBranch  s0 s1 s2 => congr_EBranch ((fun x => (Logic.eq_refl) x) s0) ((fun x => (Logic.eq_refl) x) s1) ((list_ext (@extRen_lType xilType zetalType EqlType)) s2)
     end.
 
-Definition upExt_endpoint_endpoint   (sigma : ( fin ) -> endpoint ) (tau : ( fin ) -> endpoint ) (Eq : forall x, sigma x = tau x) : forall x, (up_endpoint_endpoint sigma) x = (up_endpoint_endpoint tau) x :=
+Definition upExt_lType_lType   (sigma : ( fin ) -> lType ) (tau : ( fin ) -> lType ) (Eq : forall x, sigma x = tau x) : forall x, (up_lType_lType sigma) x = (up_lType_lType tau) x :=
   fun n => match n with
-  | S fin_n => (ap) (ren_endpoint (shift)) (Eq fin_n)
+  | S fin_n => (ap) (ren_lType (shift)) (Eq fin_n)
   | 0  => Logic.eq_refl
   end.
 
-Fixpoint ext_endpoint   (sigmaendpoint : ( fin ) -> endpoint ) (tauendpoint : ( fin ) -> endpoint ) (Eqendpoint : forall x, sigmaendpoint x = tauendpoint x) (s : endpoint ) : subst_endpoint sigmaendpoint s = subst_endpoint tauendpoint s :=
-    match s return subst_endpoint sigmaendpoint s = subst_endpoint tauendpoint s with
-    | EVar  s => Eqendpoint s
+Fixpoint ext_lType   (sigmalType : ( fin ) -> lType ) (taulType : ( fin ) -> lType ) (EqlType : forall x, sigmalType x = taulType x) (s : lType ) : subst_lType sigmalType s = subst_lType taulType s :=
+    match s return subst_lType sigmalType s = subst_lType taulType s with
+    | EVar  s => EqlType s
     | EEnd   => congr_EEnd 
-    | ERec  s0 => congr_ERec ((ext_endpoint (up_endpoint_endpoint sigmaendpoint) (up_endpoint_endpoint tauendpoint) (upExt_endpoint_endpoint (_) (_) Eqendpoint)) s0)
-    | EMsg  s0 s1 s2 s3 => congr_EMsg ((fun x => (Logic.eq_refl) x) s0) ((fun x => (Logic.eq_refl) x) s1) ((fun x => (Logic.eq_refl) x) s2) ((ext_endpoint sigmaendpoint tauendpoint Eqendpoint) s3)
-    | EBranch  s0 s1 s2 => congr_EBranch ((fun x => (Logic.eq_refl) x) s0) ((fun x => (Logic.eq_refl) x) s1) ((list_ext (ext_endpoint sigmaendpoint tauendpoint Eqendpoint)) s2)
+    | ERec  s0 => congr_ERec ((ext_lType (up_lType_lType sigmalType) (up_lType_lType taulType) (upExt_lType_lType (_) (_) EqlType)) s0)
+    | EMsg  s0 s1 s2 s3 => congr_EMsg ((fun x => (Logic.eq_refl) x) s0) ((fun x => (Logic.eq_refl) x) s1) ((fun x => (Logic.eq_refl) x) s2) ((ext_lType sigmalType taulType EqlType) s3)
+    | EBranch  s0 s1 s2 => congr_EBranch ((fun x => (Logic.eq_refl) x) s0) ((fun x => (Logic.eq_refl) x) s1) ((list_ext (ext_lType sigmalType taulType EqlType)) s2)
     end.
 
-Definition up_ren_ren_endpoint_endpoint    (xi : ( fin ) -> fin) (tau : ( fin ) -> fin) (theta : ( fin ) -> fin) (Eq : forall x, ((funcomp) tau xi) x = theta x) : forall x, ((funcomp) (upRen_endpoint_endpoint tau) (upRen_endpoint_endpoint xi)) x = (upRen_endpoint_endpoint theta) x :=
+Definition up_ren_ren_lType_lType    (xi : ( fin ) -> fin) (tau : ( fin ) -> fin) (theta : ( fin ) -> fin) (Eq : forall x, ((funcomp) tau xi) x = theta x) : forall x, ((funcomp) (upRen_lType_lType tau) (upRen_lType_lType xi)) x = (upRen_lType_lType theta) x :=
   up_ren_ren xi tau theta Eq.
 
-Fixpoint compRenRen_endpoint    (xiendpoint : ( fin ) -> fin) (zetaendpoint : ( fin ) -> fin) (rhoendpoint : ( fin ) -> fin) (Eqendpoint : forall x, ((funcomp) zetaendpoint xiendpoint) x = rhoendpoint x) (s : endpoint ) : ren_endpoint zetaendpoint (ren_endpoint xiendpoint s) = ren_endpoint rhoendpoint s :=
-    match s return ren_endpoint zetaendpoint (ren_endpoint xiendpoint s) = ren_endpoint rhoendpoint s with
-    | EVar  s => (ap) (EVar ) (Eqendpoint s)
+Fixpoint compRenRen_lType    (xilType : ( fin ) -> fin) (zetalType : ( fin ) -> fin) (rholType : ( fin ) -> fin) (EqlType : forall x, ((funcomp) zetalType xilType) x = rholType x) (s : lType ) : ren_lType zetalType (ren_lType xilType s) = ren_lType rholType s :=
+    match s return ren_lType zetalType (ren_lType xilType s) = ren_lType rholType s with
+    | EVar  s => (ap) (EVar ) (EqlType s)
     | EEnd   => congr_EEnd 
-    | ERec  s0 => congr_ERec ((compRenRen_endpoint (upRen_endpoint_endpoint xiendpoint) (upRen_endpoint_endpoint zetaendpoint) (upRen_endpoint_endpoint rhoendpoint) (up_ren_ren (_) (_) (_) Eqendpoint)) s0)
-    | EMsg  s0 s1 s2 s3 => congr_EMsg ((fun x => (Logic.eq_refl) x) s0) ((fun x => (Logic.eq_refl) x) s1) ((fun x => (Logic.eq_refl) x) s2) ((compRenRen_endpoint xiendpoint zetaendpoint rhoendpoint Eqendpoint) s3)
-    | EBranch  s0 s1 s2 => congr_EBranch ((fun x => (Logic.eq_refl) x) s0) ((fun x => (Logic.eq_refl) x) s1) ((list_comp (compRenRen_endpoint xiendpoint zetaendpoint rhoendpoint Eqendpoint)) s2)
+    | ERec  s0 => congr_ERec ((compRenRen_lType (upRen_lType_lType xilType) (upRen_lType_lType zetalType) (upRen_lType_lType rholType) (up_ren_ren (_) (_) (_) EqlType)) s0)
+    | EMsg  s0 s1 s2 s3 => congr_EMsg ((fun x => (Logic.eq_refl) x) s0) ((fun x => (Logic.eq_refl) x) s1) ((fun x => (Logic.eq_refl) x) s2) ((compRenRen_lType xilType zetalType rholType EqlType) s3)
+    | EBranch  s0 s1 s2 => congr_EBranch ((fun x => (Logic.eq_refl) x) s0) ((fun x => (Logic.eq_refl) x) s1) ((list_comp (compRenRen_lType xilType zetalType rholType EqlType)) s2)
     end.
 
-Definition up_ren_subst_endpoint_endpoint    (xi : ( fin ) -> fin) (tau : ( fin ) -> endpoint ) (theta : ( fin ) -> endpoint ) (Eq : forall x, ((funcomp) tau xi) x = theta x) : forall x, ((funcomp) (up_endpoint_endpoint tau) (upRen_endpoint_endpoint xi)) x = (up_endpoint_endpoint theta) x :=
+Definition up_ren_subst_lType_lType    (xi : ( fin ) -> fin) (tau : ( fin ) -> lType ) (theta : ( fin ) -> lType ) (Eq : forall x, ((funcomp) tau xi) x = theta x) : forall x, ((funcomp) (up_lType_lType tau) (upRen_lType_lType xi)) x = (up_lType_lType theta) x :=
   fun n => match n with
-  | S fin_n => (ap) (ren_endpoint (shift)) (Eq fin_n)
+  | S fin_n => (ap) (ren_lType (shift)) (Eq fin_n)
   | 0  => Logic.eq_refl
   end.
 
-Fixpoint compRenSubst_endpoint    (xiendpoint : ( fin ) -> fin) (tauendpoint : ( fin ) -> endpoint ) (thetaendpoint : ( fin ) -> endpoint ) (Eqendpoint : forall x, ((funcomp) tauendpoint xiendpoint) x = thetaendpoint x) (s : endpoint ) : subst_endpoint tauendpoint (ren_endpoint xiendpoint s) = subst_endpoint thetaendpoint s :=
-    match s return subst_endpoint tauendpoint (ren_endpoint xiendpoint s) = subst_endpoint thetaendpoint s with
-    | EVar  s => Eqendpoint s
+Fixpoint compRenSubst_lType    (xilType : ( fin ) -> fin) (taulType : ( fin ) -> lType ) (thetalType : ( fin ) -> lType ) (EqlType : forall x, ((funcomp) taulType xilType) x = thetalType x) (s : lType ) : subst_lType taulType (ren_lType xilType s) = subst_lType thetalType s :=
+    match s return subst_lType taulType (ren_lType xilType s) = subst_lType thetalType s with
+    | EVar  s => EqlType s
     | EEnd   => congr_EEnd 
-    | ERec  s0 => congr_ERec ((compRenSubst_endpoint (upRen_endpoint_endpoint xiendpoint) (up_endpoint_endpoint tauendpoint) (up_endpoint_endpoint thetaendpoint) (up_ren_subst_endpoint_endpoint (_) (_) (_) Eqendpoint)) s0)
-    | EMsg  s0 s1 s2 s3 => congr_EMsg ((fun x => (Logic.eq_refl) x) s0) ((fun x => (Logic.eq_refl) x) s1) ((fun x => (Logic.eq_refl) x) s2) ((compRenSubst_endpoint xiendpoint tauendpoint thetaendpoint Eqendpoint) s3)
-    | EBranch  s0 s1 s2 => congr_EBranch ((fun x => (Logic.eq_refl) x) s0) ((fun x => (Logic.eq_refl) x) s1) ((list_comp (compRenSubst_endpoint xiendpoint tauendpoint thetaendpoint Eqendpoint)) s2)
+    | ERec  s0 => congr_ERec ((compRenSubst_lType (upRen_lType_lType xilType) (up_lType_lType taulType) (up_lType_lType thetalType) (up_ren_subst_lType_lType (_) (_) (_) EqlType)) s0)
+    | EMsg  s0 s1 s2 s3 => congr_EMsg ((fun x => (Logic.eq_refl) x) s0) ((fun x => (Logic.eq_refl) x) s1) ((fun x => (Logic.eq_refl) x) s2) ((compRenSubst_lType xilType taulType thetalType EqlType) s3)
+    | EBranch  s0 s1 s2 => congr_EBranch ((fun x => (Logic.eq_refl) x) s0) ((fun x => (Logic.eq_refl) x) s1) ((list_comp (compRenSubst_lType xilType taulType thetalType EqlType)) s2)
     end.
 
-
-(*Definition up_subst_ren_gType_gType    (sigma : ( fin ) -> gType ) (zetagType : ( fin ) -> fin) (theta : ( fin ) -> gType ) (Eq : forall x, ((funcomp) (ren_gType zetagType) sigma) x = theta x) : forall x, ((funcomp) (ren_gType (upRen_gType_gType zetagType)) (up_gType_gType sigma)) x = (up_gType_gType theta) x :=
+Check compRenRen_lType. Check Logic.eq_sym. Check eq_sym.
+Definition up_subst_ren_lType_lType    (sigma : ( fin ) -> lType ) (zetalType : ( fin ) -> fin) (theta : ( fin ) -> lType ) (Eq : forall x, ((funcomp) (ren_lType zetalType) sigma) x = theta x) : 
+forall x, ((funcomp) (ren_lType (upRen_lType_lType zetalType)) (up_lType_lType sigma)) x = (up_lType_lType theta) x :=
   fun n => match n with
-  | S fin_n => (eq_trans) (compRenRen_gType (shift) (upRen_gType_gType zetagType) ((funcomp) (shift) zetagType) (fun x => Logic.eq_refl) (sigma fin_n)) 
-               ((eq_trans) ((eq_sym) (compRenRen_gType zetagType (shift) ((funcomp) (shift) zetagType) (fun x => Logic.eq_refl) (sigma fin_n))) 
-                           ((ap) (ren_gType (shift)) (Eq fin_n)))
-  | 0  => Logic.eq_refl
-  end.
-*)
-Check compRenRen_endpoint. Check Logic.eq_sym. Check eq_sym.
-Definition up_subst_ren_endpoint_endpoint    (sigma : ( fin ) -> endpoint ) (zetaendpoint : ( fin ) -> fin) (theta : ( fin ) -> endpoint ) (Eq : forall x, ((funcomp) (ren_endpoint zetaendpoint) sigma) x = theta x) : 
-forall x, ((funcomp) (ren_endpoint (upRen_endpoint_endpoint zetaendpoint)) (up_endpoint_endpoint sigma)) x = (up_endpoint_endpoint theta) x :=
-  fun n => match n with
-  | S fin_n => (eq_trans) (compRenRen_endpoint (shift) (upRen_endpoint_endpoint zetaendpoint) ((funcomp) (shift) zetaendpoint) (fun x => Logic.eq_refl) (sigma fin_n)) 
-              ((eq_trans) ((Logic.eq_sym) (compRenRen_endpoint zetaendpoint (shift) ((funcomp) (shift) zetaendpoint) (fun x => Logic.eq_refl) (sigma fin_n))) 
-                          ((ap) (ren_endpoint (shift)) (Eq fin_n)))
+  | S fin_n => (eq_trans) (compRenRen_lType (shift) (upRen_lType_lType zetalType) ((funcomp) (shift) zetalType) (fun x => Logic.eq_refl) (sigma fin_n)) 
+              ((eq_trans) ((Logic.eq_sym) (compRenRen_lType zetalType (shift) ((funcomp) (shift) zetalType) (fun x => Logic.eq_refl) (sigma fin_n))) 
+                          ((ap) (ren_lType (shift)) (Eq fin_n)))
   | 0  => Logic.eq_refl
   end.
 
-Fixpoint compSubstRen_endpoint    (sigmaendpoint : ( fin ) -> endpoint ) (zetaendpoint : ( fin ) -> fin) (thetaendpoint : ( fin ) -> endpoint ) (Eqendpoint : forall x, ((funcomp) (ren_endpoint zetaendpoint) sigmaendpoint) x = thetaendpoint x) (s : endpoint ) : ren_endpoint zetaendpoint (subst_endpoint sigmaendpoint s) = subst_endpoint thetaendpoint s :=
-    match s return ren_endpoint zetaendpoint (subst_endpoint sigmaendpoint s) = subst_endpoint thetaendpoint s with
-    | EVar  s => Eqendpoint s
+Fixpoint compSubstRen_lType    (sigmalType : ( fin ) -> lType ) (zetalType : ( fin ) -> fin) (thetalType : ( fin ) -> lType ) (EqlType : forall x, ((funcomp) (ren_lType zetalType) sigmalType) x = thetalType x) (s : lType ) : ren_lType zetalType (subst_lType sigmalType s) = subst_lType thetalType s :=
+    match s return ren_lType zetalType (subst_lType sigmalType s) = subst_lType thetalType s with
+    | EVar  s => EqlType s
     | EEnd   => congr_EEnd 
-    | ERec  s0 => congr_ERec ((compSubstRen_endpoint (up_endpoint_endpoint sigmaendpoint) (upRen_endpoint_endpoint zetaendpoint) (up_endpoint_endpoint thetaendpoint) (up_subst_ren_endpoint_endpoint (_) (_) (_) Eqendpoint)) s0)
-    | EMsg  s0 s1 s2 s3 => congr_EMsg ((fun x => (Logic.eq_refl) x) s0) ((fun x => (Logic.eq_refl) x) s1) ((fun x => (Logic.eq_refl) x) s2) ((compSubstRen_endpoint sigmaendpoint zetaendpoint thetaendpoint Eqendpoint) s3)
-    | EBranch  s0 s1 s2 => congr_EBranch ((fun x => (Logic.eq_refl) x) s0) ((fun x => (Logic.eq_refl) x) s1) ((list_comp (compSubstRen_endpoint sigmaendpoint zetaendpoint thetaendpoint Eqendpoint)) s2)
+    | ERec  s0 => congr_ERec ((compSubstRen_lType (up_lType_lType sigmalType) (upRen_lType_lType zetalType) (up_lType_lType thetalType) (up_subst_ren_lType_lType (_) (_) (_) EqlType)) s0)
+    | EMsg  s0 s1 s2 s3 => congr_EMsg ((fun x => (Logic.eq_refl) x) s0) ((fun x => (Logic.eq_refl) x) s1) ((fun x => (Logic.eq_refl) x) s2) ((compSubstRen_lType sigmalType zetalType thetalType EqlType) s3)
+    | EBranch  s0 s1 s2 => congr_EBranch ((fun x => (Logic.eq_refl) x) s0) ((fun x => (Logic.eq_refl) x) s1) ((list_comp (compSubstRen_lType sigmalType zetalType thetalType EqlType)) s2)
     end.
 
-Definition up_subst_subst_endpoint_endpoint    (sigma : ( fin ) -> endpoint ) (tauendpoint : ( fin ) -> endpoint ) (theta : ( fin ) -> endpoint ) (Eq : forall x, ((funcomp) (subst_endpoint tauendpoint) sigma) x = theta x) : forall x, ((funcomp) (subst_endpoint (up_endpoint_endpoint tauendpoint)) (up_endpoint_endpoint sigma)) x = (up_endpoint_endpoint theta) x :=
+Definition up_subst_subst_lType_lType    (sigma : ( fin ) -> lType ) (taulType : ( fin ) -> lType ) (theta : ( fin ) -> lType ) (Eq : forall x, ((funcomp) (subst_lType taulType) sigma) x = theta x) : forall x, ((funcomp) (subst_lType (up_lType_lType taulType)) (up_lType_lType sigma)) x = (up_lType_lType theta) x :=
   fun n => match n with
-  | S fin_n => (eq_trans) (compRenSubst_endpoint (shift) (up_endpoint_endpoint tauendpoint) ((funcomp) (up_endpoint_endpoint tauendpoint) (shift)) (fun x => Logic.eq_refl) (sigma fin_n)) ((eq_trans) ((Logic.eq_sym) (compSubstRen_endpoint tauendpoint (shift) ((funcomp) (ren_endpoint (shift)) tauendpoint) (fun x => Logic.eq_refl) (sigma fin_n))) ((ap) (ren_endpoint (shift)) (Eq fin_n)))
+  | S fin_n => (eq_trans) (compRenSubst_lType (shift) (up_lType_lType taulType) ((funcomp) (up_lType_lType taulType) (shift)) (fun x => Logic.eq_refl) (sigma fin_n)) ((eq_trans) ((Logic.eq_sym) (compSubstRen_lType taulType (shift) ((funcomp) (ren_lType (shift)) taulType) (fun x => Logic.eq_refl) (sigma fin_n))) ((ap) (ren_lType (shift)) (Eq fin_n)))
   | 0  => Logic.eq_refl
   end.
 
-Fixpoint compSubstSubst_endpoint    (sigmaendpoint : ( fin ) -> endpoint ) (tauendpoint : ( fin ) -> endpoint ) (thetaendpoint : ( fin ) -> endpoint ) (Eqendpoint : forall x, ((funcomp) (subst_endpoint tauendpoint) sigmaendpoint) x = thetaendpoint x) (s : endpoint ) : subst_endpoint tauendpoint (subst_endpoint sigmaendpoint s) = subst_endpoint thetaendpoint s :=
-    match s return subst_endpoint tauendpoint (subst_endpoint sigmaendpoint s) = subst_endpoint thetaendpoint s with
-    | EVar  s => Eqendpoint s
+Fixpoint compSubstSubst_lType    (sigmalType : ( fin ) -> lType ) (taulType : ( fin ) -> lType ) (thetalType : ( fin ) -> lType ) (EqlType : forall x, ((funcomp) (subst_lType taulType) sigmalType) x = thetalType x) (s : lType ) : subst_lType taulType (subst_lType sigmalType s) = subst_lType thetalType s :=
+    match s return subst_lType taulType (subst_lType sigmalType s) = subst_lType thetalType s with
+    | EVar  s => EqlType s
     | EEnd   => congr_EEnd 
-    | ERec  s0 => congr_ERec ((compSubstSubst_endpoint (up_endpoint_endpoint sigmaendpoint) (up_endpoint_endpoint tauendpoint) (up_endpoint_endpoint thetaendpoint) (up_subst_subst_endpoint_endpoint (_) (_) (_) Eqendpoint)) s0)
-    | EMsg  s0 s1 s2 s3 => congr_EMsg ((fun x => (Logic.eq_refl) x) s0) ((fun x => (Logic.eq_refl) x) s1) ((fun x => (Logic.eq_refl) x) s2) ((compSubstSubst_endpoint sigmaendpoint tauendpoint thetaendpoint Eqendpoint) s3)
-    | EBranch  s0 s1 s2 => congr_EBranch ((fun x => (Logic.eq_refl) x) s0) ((fun x => (Logic.eq_refl) x) s1) ((list_comp (compSubstSubst_endpoint sigmaendpoint tauendpoint thetaendpoint Eqendpoint)) s2)
+    | ERec  s0 => congr_ERec ((compSubstSubst_lType (up_lType_lType sigmalType) (up_lType_lType taulType) (up_lType_lType thetalType) (up_subst_subst_lType_lType (_) (_) (_) EqlType)) s0)
+    | EMsg  s0 s1 s2 s3 => congr_EMsg ((fun x => (Logic.eq_refl) x) s0) ((fun x => (Logic.eq_refl) x) s1) ((fun x => (Logic.eq_refl) x) s2) ((compSubstSubst_lType sigmalType taulType thetalType EqlType) s3)
+    | EBranch  s0 s1 s2 => congr_EBranch ((fun x => (Logic.eq_refl) x) s0) ((fun x => (Logic.eq_refl) x) s1) ((list_comp (compSubstSubst_lType sigmalType taulType thetalType EqlType)) s2)
     end.
 
-Definition rinstInst_up_endpoint_endpoint   (xi : ( fin ) -> fin) (sigma : ( fin ) -> endpoint ) (Eq : forall x, ((funcomp) (EVar ) xi) x = sigma x) : forall x, ((funcomp) (EVar ) (upRen_endpoint_endpoint xi)) x = (up_endpoint_endpoint sigma) x :=
+Definition rinstInst_up_lType_lType   (xi : ( fin ) -> fin) (sigma : ( fin ) -> lType ) (Eq : forall x, ((funcomp) (EVar ) xi) x = sigma x) : forall x, ((funcomp) (EVar ) (upRen_lType_lType xi)) x = (up_lType_lType sigma) x :=
   fun n => match n with
-  | S fin_n => (ap) (ren_endpoint (shift)) (Eq fin_n)
+  | S fin_n => (ap) (ren_lType (shift)) (Eq fin_n)
   | 0  => Logic.eq_refl
   end.
 
-Fixpoint rinst_inst_endpoint   (xiendpoint : ( fin ) -> fin) (sigmaendpoint : ( fin ) -> endpoint ) (Eqendpoint : forall x, ((funcomp) (EVar ) xiendpoint) x = sigmaendpoint x) (s : endpoint ) : ren_endpoint xiendpoint s = subst_endpoint sigmaendpoint s :=
-    match s return ren_endpoint xiendpoint s = subst_endpoint sigmaendpoint s with
-    | EVar  s => Eqendpoint s
+Fixpoint rinst_inst_lType   (xilType : ( fin ) -> fin) (sigmalType : ( fin ) -> lType ) (EqlType : forall x, ((funcomp) (EVar ) xilType) x = sigmalType x) (s : lType ) : ren_lType xilType s = subst_lType sigmalType s :=
+    match s return ren_lType xilType s = subst_lType sigmalType s with
+    | EVar  s => EqlType s
     | EEnd   => congr_EEnd 
-    | ERec  s0 => congr_ERec ((rinst_inst_endpoint (upRen_endpoint_endpoint xiendpoint) (up_endpoint_endpoint sigmaendpoint) (rinstInst_up_endpoint_endpoint (_) (_) Eqendpoint)) s0)
-    | EMsg  s0 s1 s2 s3 => congr_EMsg ((fun x => (Logic.eq_refl) x) s0) ((fun x => (Logic.eq_refl) x) s1) ((fun x => (Logic.eq_refl) x) s2) ((rinst_inst_endpoint xiendpoint sigmaendpoint Eqendpoint) s3)
-    | EBranch  s0 s1 s2 => congr_EBranch ((fun x => (Logic.eq_refl) x) s0) ((fun x => (Logic.eq_refl) x) s1) ((list_ext (rinst_inst_endpoint xiendpoint sigmaendpoint Eqendpoint)) s2)
+    | ERec  s0 => congr_ERec ((rinst_inst_lType (upRen_lType_lType xilType) (up_lType_lType sigmalType) (rinstInst_up_lType_lType (_) (_) EqlType)) s0)
+    | EMsg  s0 s1 s2 s3 => congr_EMsg ((fun x => (Logic.eq_refl) x) s0) ((fun x => (Logic.eq_refl) x) s1) ((fun x => (Logic.eq_refl) x) s2) ((rinst_inst_lType xilType sigmalType EqlType) s3)
+    | EBranch  s0 s1 s2 => congr_EBranch ((fun x => (Logic.eq_refl) x) s0) ((fun x => (Logic.eq_refl) x) s1) ((list_ext (rinst_inst_lType xilType sigmalType EqlType)) s2)
     end.
 
-Lemma rinstInst_endpoint   (xiendpoint : ( fin ) -> fin) : ren_endpoint xiendpoint = subst_endpoint ((funcomp) (EVar ) xiendpoint) .
-Proof. exact ((FunctionalExtensionality.functional_extensionality _ _ ) (fun x => rinst_inst_endpoint xiendpoint (_) (fun n => Logic.eq_refl) x)). Qed.
+Lemma rinstInst_lType   (xilType : ( fin ) -> fin) : ren_lType xilType = subst_lType ((funcomp) (EVar ) xilType) .
+Proof. exact ((FunctionalExtensionality.functional_extensionality _ _ ) (fun x => rinst_inst_lType xilType (_) (fun n => Logic.eq_refl) x)). Qed.
 
-Lemma instId_endpoint  : subst_endpoint (EVar ) = id .
-Proof. exact ((FunctionalExtensionality.functional_extensionality _ _ ) (fun x => idSubst_endpoint (EVar ) (fun n => Logic.eq_refl) ((id) x))). Qed.
+Lemma instId_lType  : subst_lType (EVar ) = id .
+Proof. exact ((FunctionalExtensionality.functional_extensionality _ _ ) (fun x => idSubst_lType (EVar ) (fun n => Logic.eq_refl) ((id) x))). Qed.
 
-Lemma rinstId_endpoint  : @ren_endpoint   (id) = id .
-Proof. exact ((eq_trans) (rinstInst_endpoint ((id) (_))) instId_endpoint). Qed.
+Lemma rinstId_lType  : @ren_lType   (id) = id .
+Proof. exact ((eq_trans) (rinstInst_lType ((id) (_))) instId_lType). Qed.
 
-Lemma varL_endpoint   (sigmaendpoint : ( fin ) -> endpoint ) : (funcomp) (subst_endpoint sigmaendpoint) (EVar ) = sigmaendpoint .
+Lemma varL_lType   (sigmalType : ( fin ) -> lType ) : (funcomp) (subst_lType sigmalType) (EVar ) = sigmalType .
 Proof. exact ((FunctionalExtensionality.functional_extensionality _ _ ) (fun x => Logic.eq_refl)). Qed.
 
-Lemma varLRen_endpoint   (xiendpoint : ( fin ) -> fin) : (funcomp) (ren_endpoint xiendpoint) (EVar ) = (funcomp) (EVar ) xiendpoint .
+Lemma varLRen_lType   (xilType : ( fin ) -> fin) : (funcomp) (ren_lType xilType) (EVar ) = (funcomp) (EVar ) xilType .
 Proof. exact ((FunctionalExtensionality.functional_extensionality _ _ ) (fun x => Logic.eq_refl)). Qed.
 
-Lemma compComp_endpoint    (sigmaendpoint : ( fin ) -> endpoint ) (tauendpoint : ( fin ) -> endpoint ) (s : endpoint ) : subst_endpoint tauendpoint (subst_endpoint sigmaendpoint s) = subst_endpoint ((funcomp) (subst_endpoint tauendpoint) sigmaendpoint) s .
-Proof. exact (compSubstSubst_endpoint sigmaendpoint tauendpoint (_) (fun n => Logic.eq_refl) s). Qed.
+Lemma compComp_lType    (sigmalType : ( fin ) -> lType ) (taulType : ( fin ) -> lType ) (s : lType ) : subst_lType taulType (subst_lType sigmalType s) = subst_lType ((funcomp) (subst_lType taulType) sigmalType) s .
+Proof. exact (compSubstSubst_lType sigmalType taulType (_) (fun n => Logic.eq_refl) s). Qed.
 
-Lemma compComp'_endpoint    (sigmaendpoint : ( fin ) -> endpoint ) (tauendpoint : ( fin ) -> endpoint ) : (funcomp) (subst_endpoint tauendpoint) (subst_endpoint sigmaendpoint) = subst_endpoint ((funcomp) (subst_endpoint tauendpoint) sigmaendpoint) .
-Proof. exact ((FunctionalExtensionality.functional_extensionality _ _ ) (fun n => compComp_endpoint sigmaendpoint tauendpoint n)). Qed.
+Lemma compComp'_lType    (sigmalType : ( fin ) -> lType ) (taulType : ( fin ) -> lType ) : (funcomp) (subst_lType taulType) (subst_lType sigmalType) = subst_lType ((funcomp) (subst_lType taulType) sigmalType) .
+Proof. exact ((FunctionalExtensionality.functional_extensionality _ _ ) (fun n => compComp_lType sigmalType taulType n)). Qed.
 
-Lemma compRen_endpoint    (sigmaendpoint : ( fin ) -> endpoint ) (zetaendpoint : ( fin ) -> fin) (s : endpoint ) : ren_endpoint zetaendpoint (subst_endpoint sigmaendpoint s) = subst_endpoint ((funcomp) (ren_endpoint zetaendpoint) sigmaendpoint) s .
-Proof. exact (compSubstRen_endpoint sigmaendpoint zetaendpoint (_) (fun n => Logic.eq_refl) s). Qed.
+Lemma compRen_lType    (sigmalType : ( fin ) -> lType ) (zetalType : ( fin ) -> fin) (s : lType ) : ren_lType zetalType (subst_lType sigmalType s) = subst_lType ((funcomp) (ren_lType zetalType) sigmalType) s .
+Proof. exact (compSubstRen_lType sigmalType zetalType (_) (fun n => Logic.eq_refl) s). Qed.
 
-Lemma compRen'_endpoint    (sigmaendpoint : ( fin ) -> endpoint ) (zetaendpoint : ( fin ) -> fin) : (funcomp) (ren_endpoint zetaendpoint) (subst_endpoint sigmaendpoint) = subst_endpoint ((funcomp) (ren_endpoint zetaendpoint) sigmaendpoint) .
-Proof. exact ((FunctionalExtensionality.functional_extensionality _ _ ) (fun n => compRen_endpoint sigmaendpoint zetaendpoint n)). Qed.
+Lemma compRen'_lType    (sigmalType : ( fin ) -> lType ) (zetalType : ( fin ) -> fin) : (funcomp) (ren_lType zetalType) (subst_lType sigmalType) = subst_lType ((funcomp) (ren_lType zetalType) sigmalType) .
+Proof. exact ((FunctionalExtensionality.functional_extensionality _ _ ) (fun n => compRen_lType sigmalType zetalType n)). Qed.
 
-Lemma renComp_endpoint    (xiendpoint : ( fin ) -> fin) (tauendpoint : ( fin ) -> endpoint ) (s : endpoint ) : subst_endpoint tauendpoint (ren_endpoint xiendpoint s) = subst_endpoint ((funcomp) tauendpoint xiendpoint) s .
-Proof. exact (compRenSubst_endpoint xiendpoint tauendpoint (_) (fun n => Logic.eq_refl) s). Qed.
+Lemma renComp_lType    (xilType : ( fin ) -> fin) (taulType : ( fin ) -> lType ) (s : lType ) : subst_lType taulType (ren_lType xilType s) = subst_lType ((funcomp) taulType xilType) s .
+Proof. exact (compRenSubst_lType xilType taulType (_) (fun n => Logic.eq_refl) s). Qed.
 
-Lemma renComp'_endpoint    (xiendpoint : ( fin ) -> fin) (tauendpoint : ( fin ) -> endpoint ) : (funcomp) (subst_endpoint tauendpoint) (ren_endpoint xiendpoint) = subst_endpoint ((funcomp) tauendpoint xiendpoint) .
-Proof. exact ((FunctionalExtensionality.functional_extensionality _ _ ) (fun n => renComp_endpoint xiendpoint tauendpoint n)). Qed.
+Lemma renComp'_lType    (xilType : ( fin ) -> fin) (taulType : ( fin ) -> lType ) : (funcomp) (subst_lType taulType) (ren_lType xilType) = subst_lType ((funcomp) taulType xilType) .
+Proof. exact ((FunctionalExtensionality.functional_extensionality _ _ ) (fun n => renComp_lType xilType taulType n)). Qed.
 
-Lemma renRen_endpoint    (xiendpoint : ( fin ) -> fin) (zetaendpoint : ( fin ) -> fin) (s : endpoint ) : ren_endpoint zetaendpoint (ren_endpoint xiendpoint s) = ren_endpoint ((funcomp) zetaendpoint xiendpoint) s .
-Proof. exact (compRenRen_endpoint xiendpoint zetaendpoint (_) (fun n => Logic.eq_refl) s). Qed.
+Lemma renRen_lType    (xilType : ( fin ) -> fin) (zetalType : ( fin ) -> fin) (s : lType ) : ren_lType zetalType (ren_lType xilType s) = ren_lType ((funcomp) zetalType xilType) s .
+Proof. exact (compRenRen_lType xilType zetalType (_) (fun n => Logic.eq_refl) s). Qed.
 
-Lemma renRen'_endpoint    (xiendpoint : ( fin ) -> fin) (zetaendpoint : ( fin ) -> fin) : (funcomp) (ren_endpoint zetaendpoint) (ren_endpoint xiendpoint) = ren_endpoint ((funcomp) zetaendpoint xiendpoint) .
-Proof. exact ((FunctionalExtensionality.functional_extensionality _ _ ) (fun n => renRen_endpoint xiendpoint zetaendpoint n)). Qed.
+Lemma renRen'_lType    (xilType : ( fin ) -> fin) (zetalType : ( fin ) -> fin) : (funcomp) (ren_lType zetalType) (ren_lType xilType) = ren_lType ((funcomp) zetalType xilType) .
+Proof. exact ((FunctionalExtensionality.functional_extensionality _ _ ) (fun n => renRen_lType xilType zetalType n)). Qed.
 
-End endpoint.
+End lType.
 
 
 Section gType.
@@ -522,19 +513,19 @@ End gType.
 
 
 
-Global Instance Subst_endpoint   : Subst1 (( fin ) -> endpoint ) (endpoint ) (endpoint ) := @subst_endpoint   .
+Global Instance Subst_lType   : Subst1 (( fin ) -> lType ) (lType ) (lType ) := @subst_lType   .
 
 Global Instance Subst_gType   : Subst1 (( fin ) -> gType ) (gType ) (gType ) := @subst_gType   .
 
-Global Instance Ren_endpoint   : Ren1 (( fin ) -> fin) (endpoint ) (endpoint ) := @ren_endpoint   .
+Global Instance Ren_lType   : Ren1 (( fin ) -> fin) (lType ) (lType ) := @ren_lType   .
 
 Global Instance Ren_gType   : Ren1 (( fin ) -> fin) (gType ) (gType ) := @ren_gType   .
 
-Global Instance VarInstance_endpoint  : Var (fin) (endpoint ) := @EVar  .
+Global Instance VarInstance_lType  : Var (fin) (lType ) := @EVar  .
 
-Notation "x '__endpoint'" := (EVar x) (at level 5, format "x __endpoint") : subst_scope.
+Notation "x '__lType'" := (EVar x) (at level 5, format "x __lType") : subst_scope.
 
-Notation "x '__endpoint'" := (@ids (_) (_) VarInstance_endpoint x) (at level 5,  format "x __endpoint") : subst_scope.
+Notation "x '__lType'" := (@ids (_) (_) VarInstance_lType x) (at level 5,  format "x __lType") : subst_scope.
 
 Notation "'var'" := (EVar) ( at level 1) : subst_scope.
 
@@ -546,29 +537,29 @@ Notation "x '__gType'" := (@ids (_) (_) VarInstance_gType x) (at level 5,  forma
 
 Notation "'var'" := (GVar) ( at level 1) : subst_scope.
 
-Class Up_endpoint X Y := up_endpoint : ( X ) -> Y.
+Class Up_lType X Y := up_lType : ( X ) -> Y.
 
-Notation "↑__endpoint" := (up_endpoint)  : subst_scope.
+Notation "↑__lType" := (up_lType)  : subst_scope.
 
 Class Up_gType X Y := up_gType : ( X ) -> Y.
 
 Notation "↑__gType" := (up_gType) : subst_scope.
 
-Notation "↑__endpoint" := (up_endpoint_endpoint) : subst_scope.
+Notation "↑__lType" := (up_lType_lType) : subst_scope.
 
-Global Instance Up_endpoint_endpoint   : Up_endpoint (_) (_) := @up_endpoint_endpoint   .
+Global Instance Up_lType_lType   : Up_lType (_) (_) := @up_lType_lType   .
 
 Notation "↑__gType" := (up_gType_gType) : subst_scope.
 
 Global Instance Up_gType_gType   : Up_gType (_) (_) := @up_gType_gType   .
 
-Notation "s [e sigmaendpoint ]" := (subst_endpoint sigmaendpoint s) (at level 7, left associativity) : subst_scope.
+Notation "s [e sigmalType ]" := (subst_lType sigmalType s) (at level 7, left associativity) : subst_scope.
 
-Notation "[e sigmaendpoint ]" := (subst_endpoint sigmaendpoint) (at level 1, left associativity) : fscope.
+Notation "[e sigmalType ]" := (subst_lType sigmalType) (at level 1, left associativity) : fscope.
 
-Notation "s ⟨e xiendpoint ⟩" := (ren_endpoint xiendpoint s) (at level 7, left associativity) : subst_scope.
+Notation "s ⟨e xilType ⟩" := (ren_lType xilType s) (at level 7, left associativity) : subst_scope.
 
-Notation "⟨e xiendpoint ⟩" := (ren_endpoint xiendpoint) (at level 1, left associativity) : fscope.
+Notation "⟨e xilType ⟩" := (ren_lType xilType) (at level 1, left associativity) : fscope.
 
 Notation "s [g sigmagType ]" := (subst_gType sigmagType s) (at level 7, left associativity) : subst_scope.
 
@@ -578,15 +569,15 @@ Notation "s ⟨g xigType ⟩" := (ren_gType xigType s) (at level 7, left associa
 
 Notation "⟨g xigType ⟩" := (ren_gType xigType) (at level 1, left associativity) : fscope.
 
-Ltac auto_unfold := repeat unfold subst1,  subst2,  Subst1,  Subst2,  ids,  ren1,  ren2,  Ren1,  Ren2,  Subst_endpoint,  Subst_gType,  Ren_endpoint,  Ren_gType,  VarInstance_endpoint,  VarInstance_gType.
+Ltac auto_unfold := repeat unfold subst1,  subst2,  Subst1,  Subst2,  ids,  ren1,  ren2,  Ren1,  Ren2,  Subst_lType,  Subst_gType,  Ren_lType,  Ren_gType,  VarInstance_lType,  VarInstance_gType.
 
-Tactic Notation "auto_unfold" "sin" "*" := repeat unfold subst1,  subst2,  Subst1,  Subst2,  ids,  ren1,  ren2,  Ren1,  Ren2,  Subst_endpoint,  Subst_gType,  Ren_endpoint,  Ren_gType,  VarInstance_endpoint,  VarInstance_gType in *.
+Tactic Notation "auto_unfold" "sin" "*" := repeat unfold subst1,  subst2,  Subst1,  Subst2,  ids,  ren1,  ren2,  Ren1,  Ren2,  Subst_lType,  Subst_gType,  Ren_lType,  Ren_gType,  VarInstance_lType,  VarInstance_gType in *.
 
 Lemma comp_id : forall (A  B : Type) (f : A -> B), f >> ssrfun.id = f. 
 Proof. intros. fext. done. 
 Qed.
 
-Ltac asimpl' := repeat first [progress rewrite ?instId_endpoint| progress rewrite ?compComp_endpoint| progress rewrite ?compComp'_endpoint| progress rewrite ?instId_gType| progress rewrite ?compComp_gType| progress rewrite ?compComp'_gType| progress rewrite ?rinstId_endpoint| progress rewrite ?compRen_endpoint| progress rewrite ?compRen'_endpoint| progress rewrite ?renComp_endpoint| progress rewrite ?renComp'_endpoint| progress rewrite ?renRen_endpoint| progress rewrite ?renRen'_endpoint| progress rewrite ?rinstId_gType| progress rewrite ?compRen_gType| progress rewrite ?compRen'_gType| progress rewrite ?renComp_gType| progress rewrite ?renComp'_gType| progress rewrite ?renRen_gType| progress rewrite ?renRen'_gType| progress rewrite ?varL_endpoint| progress rewrite ?varL_gType| progress rewrite ?varLRen_endpoint| progress rewrite ?varLRen_gType| progress (unfold up_ren, upRen_endpoint_endpoint, upRen_gType_gType, up_endpoint_endpoint, up_gType_gType)| progress (cbn [subst_endpoint subst_gType ren_endpoint ren_gType] ) | progress rewrite ?comp_id |  fsimpl].
+Ltac asimpl' := repeat first [progress rewrite ?instId_lType| progress rewrite ?compComp_lType| progress rewrite ?compComp'_lType| progress rewrite ?instId_gType| progress rewrite ?compComp_gType| progress rewrite ?compComp'_gType| progress rewrite ?rinstId_lType| progress rewrite ?compRen_lType| progress rewrite ?compRen'_lType| progress rewrite ?renComp_lType| progress rewrite ?renComp'_lType| progress rewrite ?renRen_lType| progress rewrite ?renRen'_lType| progress rewrite ?rinstId_gType| progress rewrite ?compRen_gType| progress rewrite ?compRen'_gType| progress rewrite ?renComp_gType| progress rewrite ?renComp'_gType| progress rewrite ?renRen_gType| progress rewrite ?renRen'_gType| progress rewrite ?varL_lType| progress rewrite ?varL_gType| progress rewrite ?varLRen_lType| progress rewrite ?varLRen_gType| progress (unfold up_ren, upRen_lType_lType, upRen_gType_gType, up_lType_lType, up_gType_gType)| progress (cbn [subst_lType subst_gType ren_lType ren_gType] ) | progress rewrite ?comp_id |  fsimpl].
 
 Ltac asimpl := repeat try unfold_funcomp; auto_unfold sin *; asimpl'; repeat try unfold_funcomp.
 
@@ -594,9 +585,9 @@ Tactic Notation "asimpl" "sin" hyp(J) := revert J; asimpl; intros J.
 
 Tactic Notation "auto_case" := auto_case (asimpl; cbn; eauto).
 
-Ltac substify := auto_unfold; try repeat (erewrite rinstInst_endpoint); try repeat (erewrite rinstInst_gType).
+Ltac substify := auto_unfold; try repeat (erewrite rinstInst_lType); try repeat (erewrite rinstInst_gType).
 
-Ltac renamify := auto_unfold; try repeat (erewrite <- rinstInst_endpoint); try repeat (erewrite <- rinstInst_gType).
+Ltac renamify := auto_unfold; try repeat (erewrite <- rinstInst_lType); try repeat (erewrite <- rinstInst_gType).
 
 
 
